

Reinforcement Learning HW 3

Mert Bilgin (7034879)

mert.bilgin@student.uni-tuebingen.de

Lalitha Sivakumar (6300674)

lalitha.sivakumar@student.uni-tuebingen.de

Kevin Van Le (7314700)

kevin-van.le@student.uni-tuebingen.de

November 4, 2025

1 Recap

a)

b)

c)

2 TD(λ)

2.1 a)

$$\begin{aligned}G_t^{(n)} &= R_{t+1} + \gamma R_{t+2} + \cdots + \gamma^{n-1} R_{t+n} + \gamma^n V(S_{t+n}) \\G_{t+1}^{(n-1)} &= R_{t+2} + \gamma R_{t+3} + \cdots + \gamma^{n-2} R_{t+n} + \gamma^{n-1} V(S_{t+n}) \\G_t^{(n)} &= R_{t+1} + \gamma(R_{t+2} + \gamma R_{t+3} + \cdots + \gamma^{n-2} R_{t+n} + \gamma^{n-1} V(S_{t+n})) \\&= R_{t+1} + \gamma G_{t+1}^{(n-1)}\end{aligned}$$

b)

$$G_t^\lambda = (1 - \lambda) \sum_{n=1}^{\infty} \lambda^{n-1} G_t^{(n)}$$

$$\begin{aligned}\text{Using part (a), } G_t^\lambda &= (1 - \lambda) \sum_{n=1}^{\infty} \lambda^{n-1} (R_{t+1} + \gamma G_{t+1}^{(n-1)}) \\&= R_{t+1} (1 - \lambda) \sum_{n=1}^{\infty} \lambda^{n-1} + \gamma (1 - \lambda) \sum_{n=1}^{\infty} \lambda^{n-1} G_{t+1}^{(n-1)}\end{aligned}$$

By the geometric series,

$$\sum_{n=1}^{\infty} \lambda^{n-1} = \frac{1}{1 - \lambda}$$

$$\begin{aligned}
G_t^\lambda &= R_{t+1} + \gamma(1 - \lambda) \sum_{n=1}^{\infty} \lambda^{n-1} G_{t+1}^{(n-1)} \\
&= R_{t+1} + \gamma(1 - \lambda) \sum_{n=0}^{\infty} \lambda^n G_{t+1}^{(n)} \\
&= R_{t+1} + \gamma \left[(1 - \lambda) V(S_{t+1}) + \lambda G_{t+1}^\lambda \right]
\end{aligned}$$

$$\boxed{G_t^\lambda = R_{t+1} + \gamma \left[(1 - \lambda) V(S_{t+1}) + \lambda G_{t+1}^\lambda \right]}$$